balance implementation

LLVM_DS_RBT/Insert/Naive_Insert.thy
@@ -1,7 +1,6 @@
-theory Insert
-  imports Delete
+theory Naive_Insert
+  imports "../Setup"
 begin
-
 
 context rbt_impl
 begin
@@ -10,28 +9,25 @@ interpretation llvm_prim_arith_setup .
 interpretation llvm_prim_setup .
 
 
-fun rbt_insert ::
+fun rbt_naive_insert ::
   "('key::linorder, 'val) rbt \<Rightarrow> 'key \<Rightarrow> 'val \<Rightarrow> ('key, 'val) rbt"
   where
-  "rbt_insert rbt.Empty k v = Branch color.R rbt.Empty k v rbt.Empty"
-| "rbt_insert (rbt.Branch col lhs k' v' rhs) k v = (
+    "rbt_naive_insert rbt.Empty k v = Branch color.R rbt.Empty k v rbt.Empty"
+  | "rbt_naive_insert (rbt.Branch col lhs k' v' rhs) k v = (
     if k < k'
-    then rbt.Branch col (rbt_insert lhs k v) k' v' rhs
+    then rbt.Branch col (rbt_naive_insert lhs k v) k' v' rhs
     else (
       if k > k'
-      then rbt.Branch col lhs k' v' (rbt_insert rhs k v)
+      then rbt.Branch col lhs k' v' (rbt_naive_insert rhs k v)
       else rbt.Branch col lhs k' v' rhs
     )
 )"
 
-lemma "rbt_insert rbt.Empty (1::nat) 1 = 
-    Branch color.R rbt.Empty 1 1 rbt.Empty" by auto
 
-
-partial_function (M) insert :: "
+partial_function (M) naive_insert :: "
 ('ki, 'val::llvm_rep) rbti \<Rightarrow> 'ki \<Rightarrow> 'val \<Rightarrow> ('ki, 'val) rbti llM
 " where " 
-insert tree_p k v = do {
+naive_insert tree_p k v = do {
   if tree_p = null
   then do {
     new_node \<leftarrow> ll_balloc;
@@ -45,7 +41,7 @@ insert tree_p k v = do {
     k_lt \<leftarrow> lt_impl k k_old;
     if k_lt = 1
     then do {
-      new_lhs \<leftarrow> insert (rbt_node.left tree) k v;
+      new_lhs \<leftarrow> naive_insert (rbt_node.left tree) k v;
       new_tree \<leftarrow> ll_insert_value tree new_lhs 1;
       ll_store new_tree tree_p;
       return tree_p
@@ -54,7 +50,7 @@ insert tree_p k v = do {
       k_gt \<leftarrow> lt_impl k_old k;
       if k_gt = 1
       then do {
-        new_rhs \<leftarrow> insert (rbt_node.right tree) k v;       
+        new_rhs \<leftarrow> naive_insert (rbt_node.right tree) k v;       
         new_tree \<leftarrow> ll_insert_value tree new_rhs 4;
         ll_store new_tree tree_p;
         return tree_p
@@ -68,18 +64,18 @@ insert tree_p k v = do {
 }"
 
 
-lemma insert_correct:
+lemma naive_insert_correct:
   "llvm_htriple
   (\<upharpoonleft>rbt_assn tree treei ** \<upharpoonleft>key_assn k\<^sub>n ki)
-  (insert treei ki v)
-  (\<lambda>r. \<upharpoonleft>rbt_assn (rbt_insert tree k\<^sub>n v) r)"
+  (naive_insert treei ki v)
+  (\<lambda>r. \<upharpoonleft>rbt_assn (rbt_naive_insert tree k\<^sub>n v) r)"
 proof(induction tree arbitrary: treei)
   case Empty
 
   note [simp] = rbt_assn_branch_def
 
   from Empty show ?case
-    apply (subst insert.simps)
+    apply (subst naive_insert.simps)
     apply vcg
     done
 next
@@ -87,20 +83,10 @@ next
 
   note [vcg_rules] = Branch.IH
   note [simp] = rbt_assn_branch_def
-  note [vcg_normalize_simps] = rbt_node_insert_value
 
   show ?case
-    apply (subst insert.simps)
-    apply vcg_monadify
-    apply vcg
-    subgoal 
-      apply simp
-      apply vcg
-      done
-    subgoal
-      apply vcg
-      done
-    done
+    apply (subst naive_insert.simps)
+    by vcg
 qed
 
 
