LLVM_DS_RBT/Balance.thy
@@ -1,0 +1,503 @@
+theory Balance
+  imports 
+    Delete 
+    "Insert/Balance_Adapted"
+begin
+
+
+context rbt_impl
+begin
+interpretation llvm_prim_ctrl_setup .
+interpretation llvm_prim_arith_setup .
+interpretation llvm_prim_setup .
+
+
+subsection \<open>Utilities\<close>
+
+
+definition "is_red node_p \<equiv> do {
+    if node_p = null
+    then return False
+    else do {
+      node \<leftarrow> ll_load node_p;
+      return rbt_node.color node = 0
+    }
+  }"
+
+
+lemma is_red_correct [vcg_rules]:
+  "
+    llvm_htriple
+    (\<upharpoonleft>rbt_assn t ti)
+    (is_red ti)
+    (\<lambda>r. \<up>(r = rbt_is_red t) ** \<upharpoonleft>rbt_assn t ti) 
+  "
+proof(cases t)
+  case Empty
+  then show ?thesis 
+    unfolding is_red_def rbt_is_red_def
+    by vcg
+next
+  case (Branch col lhs k v rhs)
+  then show ?thesis
+    apply (simp add: rbt_assn_branch_def rbt_is_red_def is_red_def)
+    apply (cases col)
+    apply vcg
+    done
+qed
+
+
+definition "left node_p \<equiv> do {
+    node \<leftarrow> ll_load node_p;
+    return rbt_node.left node
+}"
+
+
+lemma left_correct[vcg_rules]:
+  "
+    llvm_htriple
+    (\<upharpoonleft>rbt_assn (Branch col lhs k v rhs) ni)
+    (left ni)
+    (\<lambda>lhsi.
+      EXS coli ki vi rhsi. 
+        \<upharpoonleft>ll_bpto (RBT_NODE coli lhsi ki vi rhsi) ni **
+        \<upharpoonleft>color_assn col coli **
+        \<upharpoonleft>rbt_assn lhs lhsi **
+        \<upharpoonleft>key_assn k ki **
+        \<up>(vi=v) **  
+        \<upharpoonleft>rbt_assn rhs rhsi
+    )
+  "
+  unfolding left_def
+  by vcg
+
+
+definition "right node_p \<equiv> do {
+    node \<leftarrow> ll_load node_p;
+    return rbt_node.right node
+}"
+
+
+lemma right_correct[vcg_rules]:
+  "
+    llvm_htriple
+    (\<upharpoonleft>rbt_assn (Branch col lhs k v rhs) ni)
+    (right ni)
+    (\<lambda>rhsi.
+      EXS coli lhsi ki vi. 
+        \<upharpoonleft>ll_bpto (RBT_NODE coli lhsi ki vi rhsi) ni **
+        \<upharpoonleft>color_assn col coli **
+        \<upharpoonleft>rbt_assn lhs lhsi **
+        \<upharpoonleft>key_assn k ki **
+        \<up>(vi=v) **  
+        \<upharpoonleft>rbt_assn rhs rhsi
+    )
+  "
+  unfolding right_def
+  by vcg
+
+
+definition sc_and (infixl "&&!" 64) where
+  "sc_and a b \<equiv> do {
+    a_res \<leftarrow> a;
+    if a_res
+    then do {
+       b_res \<leftarrow> b;
+       return a_res \<and> b_res
+    }
+    else return False
+  }"
+
+
+definition "new x \<equiv> do {
+    ptr \<leftarrow> ll_balloc;
+    ll_store x ptr;
+    return ptr
+  }"
+
+
+lemma new_correct [vcg_rules]:
+  "
+    llvm_htriple
+    \<box>
+    (new x)
+    (\<lambda>r. \<upharpoonleft>ll_bpto x r)
+  "
+  unfolding new_def
+  by vcg
+
+
+definition If_ll :: 
+  "bool llM \<Rightarrow> 'a llM \<Rightarrow> 'a llM \<Rightarrow> 'a llM" 
+  ("(if! (_)/ then! (_)/ else! (_))" [0, 0, 10] 10) where
+  "If_ll condf truef elsef = do {
+    cond \<leftarrow> condf;
+    if cond
+    then truef
+    else elsef
+  }"
+
+
+lemmas [simp] = If_ll_def sc_and_def
+
+
+subsection \<open>Checks\<close>
+
+
+definition "check_1 lhs_p rhs_p \<equiv> is_red lhs_p &&! is_red rhs_p"
+definition "check_2 lhs_p rhs_p \<equiv> is_red lhs_p &&! (do {l \<leftarrow> left lhs_p; is_red l})"
+definition "check_3 lhs_p rhs_p \<equiv> is_red lhs_p &&! (do {r \<leftarrow> right lhs_p; is_red r})"
+definition "check_4 lhs_p rhs_p \<equiv> is_red rhs_p &&! (do {r \<leftarrow> right rhs_p; is_red r})"
+definition "check_5 lhs_p rhs_p \<equiv> is_red rhs_p &&! (do {l \<leftarrow> left rhs_p; is_red l})"
+
+
+lemma check_1_correct [vcg_rules]:
+  "
+    llvm_htriple
+    (\<upharpoonleft>rbt_assn lhs lhsi ** \<upharpoonleft>rbt_assn rhs rhsi)
+    (check_1 lhsi rhsi)
+    (\<lambda>r. \<upharpoonleft>rbt_assn lhs lhsi ** \<upharpoonleft>rbt_assn rhs rhsi ** \<up>(r = rbt_check_1 lhs rhs))
+  "
+  unfolding rbt_check_1_def check_1_def sc_and_def
+  by vcg
+
+
+lemma check_2_correct [vcg_rules]:
+  "
+    llvm_htriple
+    (\<upharpoonleft>rbt_assn lhs lhsi ** \<upharpoonleft>rbt_assn rhs rhsi)
+    (check_2 lhsi rhsi)
+    (\<lambda>r. \<upharpoonleft>rbt_assn lhs lhsi ** \<upharpoonleft>rbt_assn rhs rhsi ** \<up>(r = rbt_check_2 lhs rhs))
+  "
+  unfolding rbt_check_2_def check_2_def sc_and_def
+  apply vcg
+  apply (erule rbt_is_red_unfold_branch)
+  apply vcg
+  subgoal
+    unfolding rbt_assn_branch_def rbt_is_red_def rbt_left_def
+    apply vcg_try_solve
+    done 
+  subgoal by vcg
+  done
+
+
+lemma check_3_correct [vcg_rules]:
+  "
+    llvm_htriple
+    (\<upharpoonleft>rbt_assn lhs lhsi ** \<upharpoonleft>rbt_assn rhs rhsi)
+    (check_3 lhsi rhsi)
+    (\<lambda>r. \<upharpoonleft>rbt_assn lhs lhsi ** \<upharpoonleft>rbt_assn rhs rhsi ** \<up>(r = rbt_check_3 lhs rhs))
+  "
+  unfolding rbt_check_3_def check_3_def sc_and_def
+  apply vcg
+  apply (erule rbt_is_red_unfold_branch)
+  apply vcg
+  subgoal
+    unfolding rbt_assn_branch_def rbt_is_red_def rbt_right_def
+    apply vcg_try_solve
+    done 
+  subgoal by vcg
+  done
+
+
+lemma check_4_correct [vcg_rules]:
+  "
+    llvm_htriple
+    (\<upharpoonleft>rbt_assn lhs lhsi ** \<upharpoonleft>rbt_assn rhs rhsi)
+    (check_4 lhsi rhsi)
+    (\<lambda>r. \<upharpoonleft>rbt_assn lhs lhsi ** \<upharpoonleft>rbt_assn rhs rhsi ** \<up>(r = rbt_check_4 lhs rhs))
+  "
+  unfolding rbt_check_4_def check_4_def sc_and_def
+  apply vcg
+  apply (erule rbt_is_red_unfold_branch)
+  apply vcg
+  subgoal
+    unfolding rbt_assn_branch_def rbt_is_red_def rbt_right_def
+    apply vcg_try_solve
+    done 
+  subgoal by vcg
+  done
+
+
+lemma check_5_correct [vcg_rules]:
+  "
+    llvm_htriple
+    (\<upharpoonleft>rbt_assn lhs lhsi ** \<upharpoonleft>rbt_assn rhs rhsi)
+    (check_5 lhsi rhsi)
+    (\<lambda>r. \<upharpoonleft>rbt_assn lhs lhsi ** \<upharpoonleft>rbt_assn rhs rhsi ** \<up>(r = rbt_check_5 lhs rhs))
+  "
+  unfolding rbt_check_5_def check_5_def sc_and_def
+  apply vcg
+  apply (erule rbt_is_red_unfold_branch)
+  apply vcg
+  subgoal
+    unfolding rbt_assn_branch_def rbt_is_red_def rbt_left_def
+    apply vcg_try_solve
+    done 
+  subgoal by vcg
+  done
+
+
+subsection \<open>Balance Cases\<close>
+
+
+definition "balance_ad_case_1 lhs_p k v rhs_p \<equiv> do {
+  lhs \<leftarrow> ll_load lhs_p;
+  rhs \<leftarrow> ll_load rhs_p;
+  case lhs of (RBT_NODE _ a w x b) \<Rightarrow>
+  case rhs of (RBT_NODE _ c y z d) \<Rightarrow>
+    do {
+      ll_store (RBT_NODE 1 a w x b) lhs_p;
+      ll_store (RBT_NODE 1 c y z d) rhs_p;
+      new (RBT_NODE 0 lhs_p k v rhs_p)
+    }
+  }"
+
+
+lemma balance_ad_case_1_correct [vcg_rules]:
+  "
+    llvm_htriple
+    (\<upharpoonleft>rbt_assn lhs lhsi ** \<upharpoonleft>rbt_assn rhs rhsi ** \<upharpoonleft>key_assn k ki ** \<up>(rbt_check_1 lhs rhs))
+    (balance_ad_case_1 lhsi ki v rhsi)
+    (\<lambda>r. \<upharpoonleft>rbt_assn (rbt_balance_ad_case_1 lhs k v rhs) r)
+  "
+  unfolding balance_ad_case_1_def rbt_balance_ad_case_1_def new_def
+  apply vcg
+  apply (erule rbt_check_1_unfold)
+  apply vcg
+  apply auto
+  unfolding rbt_assn_branch_def
+  apply vcg
+  done
+
+
+definition "balance_ad_case_2 lhs_p k v rhs_p \<equiv> do {
+  lhs \<leftarrow> ll_load lhs_p;
+  case lhs of (RBT_NODE _ llhs_p s t c) \<Rightarrow>
+  do {
+    llhs \<leftarrow> ll_load llhs_p;
+    case llhs of (RBT_NODE _ a w x b) \<Rightarrow>
+    let y = k; z = v; d = rhs_p in
+    do {
+      ll_free lhs_p;
+      ll_free llhs_p;
+      lhs_n \<leftarrow> new (RBT_NODE 1 a w x b);
+      rhs_n \<leftarrow> new (RBT_NODE 1 c y z d);
+      new (RBT_NODE 0 lhs_n s t rhs_n)
+    }
+  }
+}"
+
+
+lemma balance_ad_case_2_correct [vcg_rules]: 
+  "
+    llvm_htriple
+    (\<upharpoonleft>rbt_assn lhs lhsi ** \<upharpoonleft>rbt_assn rhs rhsi ** \<upharpoonleft>key_assn k ki ** \<up>(rbt_check_2 lhs rhs))
+    (balance_ad_case_2 lhsi ki v rhsi)
+    (\<lambda>r. \<upharpoonleft>rbt_assn (rbt_balance_ad_case_2 lhs k v rhs) r)
+  "
+  unfolding balance_ad_case_2_def rbt_balance_ad_case_2_def new_def
+  apply vcg
+  apply (erule rbt_check_2_unfold)
+  apply vcg
+  apply auto
+  unfolding rbt_assn_branch_def
+  apply vcg
+  done
+
+
+definition "balance_ad_case_3 lhs_p k v rhs_p \<equiv> do {
+  lhs \<leftarrow> ll_load lhs_p;
+  case lhs of (RBT_NODE _ a w x rlhs_p) \<Rightarrow>
+  do {
+    rlhs \<leftarrow> ll_load rlhs_p;
+    case rlhs of (RBT_NODE _ b s t c) \<Rightarrow>
+    let y = k; z = v; d = rhs_p in
+    do {
+      ll_free lhs_p;
+      ll_free rlhs_p;
+      lhs_n \<leftarrow> new (RBT_NODE 1 a w x b);
+      rhs_n \<leftarrow> new (RBT_NODE 1 c y z d);
+      new (RBT_NODE 0 lhs_n s t rhs_n)
+    }
+  }
+}"
+
+
+lemma balance_ad_case_3_correct [vcg_rules]: 
+  "
+    llvm_htriple
+    (\<upharpoonleft>rbt_assn lhs lhsi ** \<upharpoonleft>rbt_assn rhs rhsi ** \<upharpoonleft>key_assn k ki ** \<up>(rbt_check_3 lhs rhs))
+    (balance_ad_case_3 lhsi ki v rhsi)
+    (\<lambda>r. \<upharpoonleft>rbt_assn (rbt_balance_ad_case_3 lhs k v rhs) r)
+  "
+  unfolding balance_ad_case_3_def rbt_balance_ad_case_3_def new_def
+  apply vcg
+  apply (erule rbt_check_3_unfold)
+  apply vcg
+  apply auto
+  unfolding rbt_assn_branch_def
+  apply vcg
+  done
+
+
+definition "balance_ad_case_4 l_p k v r_p \<equiv> do {
+  let a=l_p; w=k; x=v in
+  do {    
+    r \<leftarrow> ll_load r_p;
+    case r of (RBT_NODE _ b s t rr_p) \<Rightarrow> 
+    do {
+      rr \<leftarrow> ll_load rr_p;
+      case rr of (RBT_NODE _ c y z d) \<Rightarrow> 
+      do {
+        ll_free r_p;
+        ll_free rr_p;
+        lhs_n \<leftarrow> new (RBT_NODE 1 a w x b);
+        rhs_n \<leftarrow> new (RBT_NODE 1 c y z d);
+        new (RBT_NODE 0 lhs_n s t rhs_n)
+      }
+    }
+  }
+}"
+
+
+lemma balance_ad_case_4_correct [vcg_rules]: 
+  "
+    llvm_htriple
+    (\<upharpoonleft>rbt_assn lhs lhsi ** \<upharpoonleft>rbt_assn rhs rhsi ** \<upharpoonleft>key_assn k ki ** \<up>(rbt_check_4 lhs rhs))
+    (balance_ad_case_4 lhsi ki v rhsi)
+    (\<lambda>r. \<upharpoonleft>rbt_assn (rbt_balance_ad_case_4 lhs k v rhs) r)
+  "
+  unfolding balance_ad_case_4_def rbt_balance_ad_case_4_def new_def
+  apply vcg
+  apply (erule rbt_check_4_unfold)
+  apply vcg
+  apply auto
+  unfolding rbt_assn_branch_def
+  apply vcg
+  done
+
+
+definition "balance_ad_case_5 l_p k v r_p \<equiv> do {
+  let a=l_p; w=k; x=v in
+  do {    
+    r \<leftarrow> ll_load r_p;
+    case r of (RBT_NODE _ rl_p y z d) \<Rightarrow> 
+    do {
+      rl \<leftarrow> ll_load rl_p;
+      case rl of (RBT_NODE _ b s t c) \<Rightarrow> 
+      do {
+        ll_free r_p;
+        ll_free rl_p;
+        lhs_n \<leftarrow> new (RBT_NODE 1 a w x b);
+        rhs_n \<leftarrow> new (RBT_NODE 1 c y z d);
+        new (RBT_NODE 0 lhs_n s t rhs_n)
+      }
+    }
+  }
+}"
+
+
+lemma balance_ad_case_5_correct [vcg_rules]: 
+  "
+    llvm_htriple
+    (\<upharpoonleft>rbt_assn lhs lhsi ** \<upharpoonleft>rbt_assn rhs rhsi ** \<upharpoonleft>key_assn k ki ** \<up>(rbt_check_5 lhs rhs))
+    (balance_ad_case_5 lhsi ki v rhsi)
+    (\<lambda>r. \<upharpoonleft>rbt_assn (rbt_balance_ad_case_5 lhs k v rhs) r)
+  "
+  unfolding balance_ad_case_5_def rbt_balance_ad_case_5_def new_def
+  apply vcg
+  apply (erule rbt_check_5_unfold)
+  apply vcg
+  apply auto
+  unfolding rbt_assn_branch_def
+  apply vcg
+  done
+
+
+definition "balance_ad_case_6 l_p k v r_p \<equiv> new (RBT_NODE 1 l_p k v r_p)"
+
+
+lemma balance_ad_case_6_correct [vcg_rules]: 
+  "
+    llvm_htriple
+    (\<upharpoonleft>rbt_assn lhs lhsi ** \<upharpoonleft>rbt_assn rhs rhsi ** \<upharpoonleft>key_assn k ki)
+    (balance_ad_case_6 lhsi ki v rhsi)
+    (\<lambda>r. \<upharpoonleft>rbt_assn (rbt_balance_ad_case_6 lhs k v rhs) r)
+  "
+  unfolding balance_ad_case_6_def rbt_balance_ad_case_6_def
+  apply vcg
+  unfolding rbt_assn_branch_def
+  by vcg
+
+
+subsection \<open>Balance Function\<close>
+
+
+definition balance ::
+  "('ki, 'v::llvm_rep) rbti \<Rightarrow> 'ki \<Rightarrow> 'v \<Rightarrow> ('ki, 'v) rbti \<Rightarrow> ('ki, 'v) rbti llM" where
+  "balance lhs_p k v rhs_p = do {
+      if! check_1 lhs_p rhs_p
+      then! balance_ad_case_1 lhs_p k v rhs_p
+      else! if! check_2 lhs_p rhs_p
+      then! balance_ad_case_2 lhs_p k v rhs_p
+      else! if! check_3 lhs_p rhs_p
+      then! balance_ad_case_3 lhs_p k v rhs_p
+      else! if! check_4 lhs_p rhs_p
+      then! balance_ad_case_4 lhs_p k v rhs_p
+      else! if! check_5 lhs_p rhs_p
+      then! balance_ad_case_5 lhs_p k v rhs_p
+      else! balance_ad_case_6 lhs_p k v rhs_p
+  }"
+
+
+lemma balance_correct:
+  "llvm_htriple
+  (
+    \<upharpoonleft>rbt_assn tree_l tree_li **
+    \<upharpoonleft>rbt_assn tree_r tree_ri **   
+    \<upharpoonleft>key_assn k ki
+  )
+  (balance tree_li ki v tree_ri)
+  (\<lambda>ri. \<upharpoonleft>rbt_assn (rbt_balance_ad tree_l k v tree_r) ri) 
+  "
+proof -
+  show ?thesis
+    unfolding balance_def
+    by vcg
+qed
+
+
+subsection \<open>WIP GARBAGE\<close>
+
+
+lemma pure_part_split_conjE:
+  fixes A B
+  assumes "pure_part (A ** B)"
+  obtains
+    "pure_part A"
+    "pure_part B"
+  using assms
+  by (blast dest: pure_part_split_conj)
+
+lemma rbt_assn_non_null_def:
+  assumes 
+    "pure_part (\<upharpoonleft>rbt_assn tree_l tree_li)"
+  shows
+    "tree_li = null \<longleftrightarrow> (tree_l = rbt.Empty)"
+  using assms
+  apply (cases tree_l)
+  subgoal by simp
+  subgoal
+    unfolding rbt_assn_branch_def
+    by fastforce
+  done
+
+lemma fri_exE: "(\<And>x. FRAME_INFER (P x) Qs F) \<Longrightarrow> FRAME_INFER (EXS x. P x) Qs F"
+  by (auto simp: FRAME_INFER_def entails_def)
+
+
+end
+
+
+end
