LLVM_DS_RBT/Insert/Balance_Adapted.thy
@@ -1,0 +1,164 @@
+theory Balance_Adapted
+  imports "HOL-Library.RBT_Impl"
+begin
+
+subsection \<open>Rbt Utilities\<close>
+
+definition "rbt_is_red tree \<equiv> 
+  case tree of
+    (Branch color.R _ _ _ _ ) \<Rightarrow> True |
+    _ \<Rightarrow> False
+"
+
+
+lemma rbt_is_red_unfold_branch:
+  assumes "rbt_is_red tree"
+  obtains lhs k v rhs where "tree = Branch color.R lhs k v rhs"
+  using assms
+  unfolding rbt_is_red_def
+  apply (cases tree)
+  subgoal by auto
+  subgoal for c  by (cases c; auto)
+  done
+
+
+definition "rbt_left node \<equiv> case node of (Branch _ lhs _ _ _) \<Rightarrow> lhs" 
+definition "rbt_right node \<equiv> case node of (Branch _ _ _ _ rhs) \<Rightarrow> rhs"
+
+
+subsection \<open>Balance Cases\<close>
+
+definition "rbt_balance_ad_case_1 lhs k v rhs \<equiv>
+  case (lhs, k, v, rhs) of 
+  ((Branch color.R a w x b), s, t, (Branch color.R c y z d)) \<Rightarrow>
+   Branch color.R (Branch color.B a w x b) s t (Branch color.B c y z d)"
+
+definition "rbt_balance_ad_case_2 lhs k v rhs \<equiv>
+  case (lhs, k, v, rhs) of 
+  ((Branch color.R (Branch color.R a w x b) s t c), y, z, d) \<Rightarrow>
+   Branch color.R (Branch color.B a w x b) s t (Branch color.B c y z d)"
+
+definition "rbt_balance_ad_case_3 lhs k v rhs \<equiv>
+  case (lhs, k, v, rhs) of 
+  ((Branch color.R a w x (Branch color.R b s t c)), y, z, d) \<Rightarrow>
+   Branch color.R (Branch color.B a w x b) s t (Branch color.B c y z d)"
+
+definition "rbt_balance_ad_case_4 lhs k v rhs \<equiv>
+  case (lhs, k, v, rhs) of 
+  (a, w, x, (Branch color.R b s t (Branch color.R c y z d))) \<Rightarrow>
+   Branch color.R (Branch color.B a w x b) s t (Branch color.B c y z d)"
+
+definition "rbt_balance_ad_case_5 lhs k v rhs \<equiv>
+  case (lhs, k, v, rhs) of 
+  (a, w, x, (Branch color.R (Branch color.R b s t c) y z d)) \<Rightarrow>
+   Branch color.R (Branch color.B a w x b) s t (Branch color.B c y z d)"
+
+definition "rbt_balance_ad_case_6 lhs k v rhs \<equiv>
+  case (lhs, k, v, rhs) of 
+  (a, s, t, b) \<Rightarrow> Branch color.B a s t b"
+
+
+subsection \<open>Case Checks\<close>
+
+
+definition "rbt_check_1 lhs rhs \<equiv> rbt_is_red lhs \<and> rbt_is_red rhs"
+definition "rbt_check_2 lhs rhs \<equiv> rbt_is_red lhs \<and> rbt_is_red (rbt_left lhs)"
+definition "rbt_check_3 lhs rhs \<equiv> rbt_is_red lhs \<and> rbt_is_red (rbt_right lhs)"
+definition "rbt_check_4 lhs rhs \<equiv> rbt_is_red rhs \<and> rbt_is_red (rbt_right rhs)"
+definition "rbt_check_5 lhs rhs \<equiv> rbt_is_red rhs \<and> rbt_is_red (rbt_left rhs)"
+
+
+subsubsection \<open>unfold lemmas for checks\<close>
+
+
+lemma rbt_check_1_unfold:
+  assumes "rbt_check_1 lhs rhs"
+  obtains ll k_l v_l lr
+    rl k_r v_r rr where
+    "lhs = (Branch color.R ll k_l v_l lr)"
+    "rhs = (Branch color.R rl k_r v_r rr)"
+  using assms by (meson rbt_is_red_unfold_branch rbt_check_1_def)
+
+
+lemma rbt_check_2_unfold:
+  assumes "rbt_check_2 lhs rhs"
+  obtains k_l v_l lr
+    lll k_ll v_ll llr where
+    "lhs = (Branch color.R (Branch color.R lll k_ll v_ll llr) k_l v_l lr)"
+  using assms
+  unfolding rbt_check_2_def rbt_left_def
+  by (fastforce elim: rbt_is_red_unfold_branch)
+
+
+lemma rbt_check_3_unfold:
+  assumes "rbt_check_3 lhs rhs"
+  obtains ll k_l v_l
+    lrl k_lr v_lr lrr where
+    "lhs = (Branch color.R ll k_l v_l (Branch color.R lrl k_lr v_lr lrr))"
+  using assms
+  unfolding rbt_check_3_def rbt_right_def
+  by (fastforce elim: rbt_is_red_unfold_branch)
+
+
+lemma rbt_check_4_unfold:
+  assumes "rbt_check_4 lhs rhs"
+  obtains rl k_r v_r
+    rrl k_rr v_rr rrr where
+    "rhs = (Branch color.R rl k_r v_r (Branch color.R rrl k_rr v_rr rrr))"
+  using assms
+  unfolding rbt_check_4_def rbt_right_def
+  by (fastforce elim: rbt_is_red_unfold_branch)
+
+
+lemma rbt_check_5_unfold:
+  assumes "rbt_check_5 lhs rhs"
+  obtains k_r v_r rr
+    rll k_rl v_rl rlr where
+    "rhs = (Branch color.R (Branch color.R rll k_rl v_rl rlr) k_r v_r rr)"
+  using assms
+  unfolding rbt_check_5_def rbt_left_def
+  by (fastforce elim: rbt_is_red_unfold_branch)
+
+
+subsubsection \<open>Adapted Balance Function\<close>
+
+fun rbt_balance_ad where 
+  "rbt_balance_ad lhs k v rhs = 
+  (
+    if rbt_check_1 lhs rhs
+      then rbt_balance_ad_case_1 lhs k v rhs
+    else if rbt_check_2 lhs rhs
+      then rbt_balance_ad_case_2 lhs k v rhs
+    else if rbt_check_3 lhs rhs
+      then rbt_balance_ad_case_3 lhs k v rhs
+    else if rbt_check_4 lhs rhs
+      then rbt_balance_ad_case_4 lhs k v rhs
+    else if rbt_check_5 lhs rhs
+      then rbt_balance_ad_case_5 lhs k v rhs
+    else rbt_balance_ad_case_6 lhs k v rhs
+  )
+  "
+
+
+lemma rbt_balance_ad_correct: 
+  "rbt_balance_ad lhs k v rhs = balance lhs k v rhs"
+  apply (induction lhs k v rhs rule: balance.induct)
+  by(auto simp add: 
+      rbt_is_red_def
+      rbt_left_def
+      rbt_right_def
+      rbt_balance_ad_case_1_def
+      rbt_balance_ad_case_2_def
+      rbt_balance_ad_case_3_def
+      rbt_balance_ad_case_4_def
+      rbt_balance_ad_case_5_def
+      rbt_balance_ad_case_6_def
+      rbt_check_1_def
+      rbt_check_2_def
+      rbt_check_3_def
+      rbt_check_4_def
+      rbt_check_5_def
+      )
+
+
+end
